pcuic/theories/PCUICAstUtils.v
@@ -11,6 +11,9 @@ Derive Signature for All All2.
 Definition string_of_aname (b : binder_annot name) :=
   string_of_name b.(binder_name).
 
+Definition string_of_float64_model (f : float64_model) := 
+  "<float>".
+
 Fixpoint string_of_term (t : term) :=
   match t with
   | tRel n => "Rel(" ^ string_of_nat n ^ ")"
@@ -36,6 +39,8 @@ Fixpoint string_of_term (t : term) :=
             ^ string_of_term c ^ ")"
   | tFix l n => "Fix(" ^ (string_of_list (string_of_def string_of_term) l) ^ "," ^ string_of_nat n ^ ")"
   | tCoFix l n => "CoFix(" ^ (string_of_list (string_of_def string_of_term) l) ^ "," ^ string_of_nat n ^ ")"
+  | tInt n => "Int(" ^ string_of_Z (proj1_sig n) ^ ")"
+  | tFloat f => "Float(" ^ string_of_float64_model f ^ ")"
   end.
 
 Lemma lookup_env_nil c s : lookup_env [] c = Some s -> False.
