pcuic/theories/PCUICInversion.v
@@ -239,6 +239,21 @@ Section Inversion.
     intros Γ mfix idx T h. invtac h.
   Qed.
 
+  (** At this stage we don't typecheck primitive types *)
+  Lemma inversion_Int :
+    forall {Γ i T},
+      Σ ;;; Γ |- tInt i : T -> False.
+  Proof.
+    intros Γ i T h. now depind h.
+  Qed.
+
+  Lemma inversion_Float :
+    forall {Γ f T},
+      Σ ;;; Γ |- tFloat f : T -> False.
+  Proof.
+    intros Γ i T h. now depind h.
+  Qed.
+
   Lemma inversion_it_mkLambda_or_LetIn :
     forall {Γ Δ t T},
       Σ ;;; Γ |- it_mkLambda_or_LetIn Δ t : T ->
